chore: Sid just realized that we don't have bitwise ops defined for Int. WTF!

SSA/Experimental/Bits/Fast/MBA.lean
@@ -1,3 +1,5 @@
+import Lean
+
 @[simp]
 theorem BitVec.zero_concat (b : Bool) : (0#0).concat b = BitVec.ofBool b := by
   apply BitVec.eq_of_getLsbD_eq
@@ -12,25 +14,109 @@ theorem BitVec.intCast_zero : ((0 : Int) : BitVec w) = 0#w := by simp
 namespace MBA
 
 inductive Factor 
-| term (n : Nat)
+| var (n : Nat)
 | and (x y : Factor) 
 | or (x y : Factor) 
 | xor (x y : Factor) 
 | not (x : Factor) 
 
+def Factor.numVars : Factor → Nat
+| .var n => n+1
+| .and x y | .or x y | xor x y => max (x.numVars) (y.numVars)
+| .not x => x.numVars
+
+@[simp]
+theorem Factor.numVars_term : (Factor.var n).numVars = n + 1 := rfl
+
 def Env (w : Nat) := List (BitVec w)
 def Env.getLsb (env : Env w) : Env 1 := env.map <| fun x => BitVec.ofBool <| x.getLsbD 0
 def Env.getNonLsbs (env : Env w) : Env (w-1) := env.map <| fun x => x.extractLsb' 1 (w-1)
   
-
 def Factor.reflect {w : Nat} (xs : Env w) : Factor → BitVec w 
-| .term n => xs.getD n (0#w)
+| .var n => xs.getD n (0#w)
 | .and x y => x.reflect xs &&& y.reflect xs
 | .or x y => x.reflect xs ||| y.reflect xs
 | .xor x y => x.reflect xs ^^^ y.reflect xs
 | .not x => ~~~ (x.reflect xs)
 
-def Factor.denote {w : Nat} (xs : Env w) (f : Factor) : Int := f.reflect xs |>.toInt
+
+def Factor.denote {w : Nat} (xs : Env w) (f : Factor) : Int := 
+  match f with 
+  | .var n => xs.getD n (0#w) |>.toInt 
+  | .and x y => (x.denote xs) && (y.denote xs)
+
+def Factor.denote_eq_toInt_reflect {w : Nat} (xs : Env w) (f : Factor) : f.denote xs = (f.reflect xs |>.toInt) := by sorry
+
+
+/-- Split a denote at an env intoa denote at the LSB and the denote at the non-Lsbs -/
+theorem Factor.denote_eq_add_denote_getLsb_denote_getNonLsbs (x : Factor) (xs : Env w) : 
+    x.denote env = 2 * x.denote xs.getNonLsbs  + x.denote xs.getLsb := by
+  induction x generalizing xs 
+  case var n => sorry
+  case and x y hx hy =>
+  sorry
+
+
+
+/--
+Environment of *finite* size, which can agree with the `Factor.reflect`. 
+We need `Factor.reflectFin` to show that our brute-force evaluation for length 1 has a finite environment size for exhaustive enumeration,
+We need `Factor.reflect` to def-eq-unify with the user's given goal state.
+We show their equivalence to allow us to decide on `denoteFin`, and to use this when proving facts about `denote`.
+-/
+def EnvFin (w : Nat) (n : Nat) := Fin n → (BitVec w)
+
+def Factor.reflectFin {w : Nat} (f : Factor) (xs : EnvFin w f.numVars) : BitVec w := 
+  match f with
+  | .var n => xs ⟨n, by simp⟩
+  | .and x y => 
+    x.reflectFin (fun n => xs ⟨n, by simp [numVars]; omega⟩) &&& y.reflectFin (fun n => xs ⟨n, by simp [numVars]; omega⟩)
+  | .or x y => 
+     x.reflectFin (fun n => xs ⟨n, by simp [numVars]; omega⟩) ||| y.reflectFin (fun n => xs ⟨n, by simp [numVars]; omega⟩) 
+  | .xor x y => 
+     x.reflectFin (fun n => xs ⟨n, by simp [numVars]; omega⟩) ^^^ y.reflectFin (fun n => xs ⟨n, by simp [numVars]; omega⟩) 
+  | .not x => 
+     ~~~ x.reflectFin (fun n => xs ⟨n, by simp [numVars]⟩) 
+
+/-- Show that reflect and reflectFin agree in their values -/
+theorem Factor.reflect_eq_reflectFin {f : Factor} {xs : List (BitVec w)} {xsFin : EnvFin w f.numVars} (h : ∀ (i : Fin f.numVars), xs[i]?.getD 0#w = xsFin i) :
+    f.reflect xs = f.reflectFin xsFin := by
+  induction f 
+  case var n => simp [reflect, reflectFin] at h ⊢; rw[← h] 
+  case and x y hx hy => 
+    simp [reflect, reflectFin] at h ⊢
+    rw[← hx, ← hy]
+    · intros i 
+      simp [← h]
+    · intros i 
+      simp [← h]
+  case or x y hx hy => 
+    simp [reflect, reflectFin] at h ⊢
+    rw[← hx, ← hy]
+    · intros i 
+      simp [← h]
+    · intros i 
+      simp [← h]
+  case xor x y hx hy => 
+    simp [reflect, reflectFin] at h ⊢
+    rw[← hx, ← hy]
+    · intros i 
+      simp [← h]
+    · intros i 
+      simp [← h]
+  case not x hx => 
+    simp [reflect, reflectFin] at h ⊢
+    rw[← hx]
+    · intros i 
+      simp [← h]
+
+
+def Factor.denoteFin {w : Nat} (f : Factor) (xs : EnvFin w f.numVars) : Int := f.reflectFin xs |>.toInt
+
+/-- Show that 'denote'  agrees with 'denoteFin' -/
+theorem Factor.denoteFin_eq_denote {f : Factor} {xs : List (BitVec w)} {xsFin : EnvFin w f.numVars} (h : ∀ (i : Fin f.numVars), xs[i]?.getD 0#w = xsFin i) :
+    f.denoteFin xsFin = f.denote xs := by 
+  rw [Factor.denote, Factor.denoteFin, Factor.reflect_eq_reflectFin h]
 
 theorem Factor.reflect_eq_ofInt_denote {w : Nat} (xs : Env w) (f : Factor) : 
     f.reflect xs = (BitVec.ofInt w <| f.denote xs) := by
@@ -43,10 +129,12 @@ theorem Factor.reflect_zero_of_denote_zero {w : Nat} {f : Factor} {xs : Env w} (
 
 
 @[simp]
-theorem Factor.reflect_width_zero  (f : Factor) (env : Env 0) : 
-   f.reflect env = 0#0 := by
+theorem Factor.reflect_width_zero  (f : Factor) (env : Env 0) : f.reflect env = 0#0 := by
   apply Subsingleton.elim
 
+@[simp]
+theorem Factor.denote_width_zero  (f : Factor) (env : Env 0) : f.denote env = 0 := by
+  simp [denote]
 
 structure Term where 
   c : Int
@@ -58,6 +146,15 @@ def Term.reflect {w : Nat}  (t : Term) (xs: Env w) : BitVec w :=
 
 def Term.denote {w : Nat} (t : Term) (xs : Env w) : Int := 
   t.c * t.f.denote xs
+
+def Term.numVars (t : Term) : Nat := t.f.numVars
+
+def Term.denoteFin {w : Nat} (t : Term) (xsFin: EnvFin w t.numVars) : Int :=
+  t.c * t.f.denoteFin xsFin
+
+theorem Term.denoteFin_eq_denote {t : Term} {xs : List (BitVec w)} {xsFin : EnvFin w t.numVars} (h : ∀ (i : Fin t.numVars), xs[i]?.getD 0#w = xsFin i) :
+    t.denoteFin xsFin = t.denote xs := by 
+  simp [Term.denoteFin, Term.denote, Factor.denoteFin_eq_denote h]
 
 
 @[simp]
@@ -77,12 +174,22 @@ theorem Term.reflect_zero_of_denote_zero {w : Nat} {t : Term} {xs : Env w} (h : 
 theorem Term.reflect_width_zero  (t : Term) (env : Env 0) : 
     t.reflect env = 0 := by simp [Term.reflect]
 
+@[simp]
+theorem Term.denote_width_zero  (t : Term) (env : Env 0) : 
+    t.denote env = 0 := by simp [Term.denote]
+
 def Eqn := List Term
+
+def Eqn.numVars (e : Eqn) : Nat := 
+  match e with 
+  | [] => 0 
+  | e :: es => max e.numVars (Eqn.numVars es)
 
 def Eqn.reflect {w : Nat} (e : Eqn) (env : Env w) : BitVec w := 
   match e with
   | [] => 0
   | t :: ts => t.reflect env + Eqn.reflect ts env
+
 
 @[simp]
 theorem Eqn.reflect_nil  {w : Nat} (env : Env w) : 
@@ -108,6 +215,28 @@ theorem Eqn.denote_cons {w : Nat}
     (t : Term) (ts : List Term) (env : Env w) : 
     Eqn.denote (t :: ts) env = t.denote env + Eqn.denote ts env := rfl
 
+def Eqn.denoteFin {w : Nat} (e : Eqn) (envFin : EnvFin w e.numVars) : Int := 
+  match e with
+  | [] => 0
+  | t :: ts => t.denoteFin (fun n => envFin ⟨n, by simp [Eqn.numVars]; omega⟩) + Eqn.denoteFin ts (fun n => envFin ⟨n, by simp [Eqn.numVars]; omega⟩)
+
+/- To evaluate `e.denote`, one can equally well evaluate `e.denoteFin` -/
+theorem Eqn.denoteFin_eq_denote {e : Eqn} {xs : List (BitVec w)} {xsFin : EnvFin w e.numVars} (h : ∀ (i : Fin e.numVars), xs[i]?.getD 0#w = xsFin i) :
+    e.denoteFin xsFin = e.denote xs := by 
+  induction e 
+  case nil => simp [Eqn.denoteFin]
+  case cons t es ih => 
+    simp [Eqn.denoteFin]
+    rw [Term.denoteFin_eq_denote (xs := xs)]
+    · simp
+      rw [ih]
+      · intros i 
+        rw [← h]
+        simp
+    · intros i
+      rw [← h]
+      simp
+       
 @[simp]
 theorem Eqn.reflect_width_zero  (es : Eqn) (env : Env 0) : 
     Eqn.reflect es env = 0 := by 
@@ -115,7 +244,17 @@ theorem Eqn.reflect_width_zero  (es : Eqn) (env : Env 0) :
   case nil => simp [Eqn.reflect]
   case cons e es ih => 
     simp [ih, Eqn.reflect]
-    apply Subsingleton.elim
+
+
+@[simp]
+theorem Eqn.denote_width_zero  (es : Eqn) (env : Env 0) : 
+    Eqn.denote es env = 0 := by 
+  induction es 
+  case nil => simp [Eqn.denote]
+  case cons e es ih => 
+    simp [ih, Eqn.denote]
+
+
 
 @[simp]
 theorem Eqn.reflect_eq_ofInt_denote {w : Nat} (xs : Env w) (e : Eqn) :
@@ -125,8 +264,6 @@ theorem Eqn.reflect_eq_ofInt_denote {w : Nat} (xs : Env w) (e : Eqn) :
   case cons t ts ih => 
     simp 
     simp [BitVec.ofInt_add, ih]
-
-
 @[simp]
 theorem Eqn.reflect_zero_of_denote_zero {w : Nat} (xs : Env w) (e : Eqn) (h : e.denote xs = 0) :
     e.reflect xs = 0 := by simp [h]
@@ -138,26 +275,51 @@ def Env.getLsb_eq_of_width_one (env : List (BitVec 1)) : Env.getLsb env = env :=
   ext x i hi
   have : i = 0 := by omega
   simp [this]
+
+
+theorem Eqn.denote_hard_case (e : Eqn) (h : ∀ (env1 : List (BitVec 1)), Eqn.denote e env1 = 0) :
+    ∀ {w : Nat} (env : List (BitVec w)), e.denote env = 0 := by
+  intros w env 
+  induction w 
+  case zero => simp
+  case succ w ih =>
+    induction e 
+    case nil => simp
+    case cons t es ih' =>
+      simp
+
+
   
       
-theorem Eqn.denote_hard_case (e : Eqn) (h : ∀ (env1 : List (BitVec 1)), Eqn.reflect e env1 = 0) :
+theorem Eqn.denote_hard_case (e : Eqn) (h : ∀ (env1 : List (BitVec 1)), Eqn.denote e env1 = 0) :
     ∀ {w : Nat} (env : List (BitVec w)), e.reflect env = 0 := by
   intros w env 
   induction w 
   case zero => simp
   case succ w ih =>
+    rw [Eqn.reflect_eq_ofInt_denote]
+    induction e 
+    case nil => simp
+    case cons t es ih =>
     sorry
 
-theorem Eqn.denote_iff_denote_one (e : Eqn) : 
-    (∀ (w : Nat) (env : List (BitVec w)), Eqn.reflect e env = 0) ↔ 
-    (∀ env1 : List (BitVec 1), Eqn.reflect e env1 = 0) := by
-  constructor 
-  · intros h
-    apply h
-  · intros h
-    intros w env
-    rw [Eqn.denote_hard_case]
-    exact h
+/-
+instance decEqnDenoteFinWidth1 {e : Eqn} : Decidable (∀ env1 : Env (BitVec 1), Eqn.denoteFin e env1 = 0) := 
+  sorry
+
+instance {e : Eqn} : Decidable (∀ env1 : List (BitVec 1), Eqn.denote e env1 = 0) := 
+  sorry
+-/
+  
+
+/--
+Central theorem: To decide if a bitvector equation is zero for all widths, it sufficest to check that the denotation is zero at width zero.
+-/
+theorem Eqn.forall_width_reflect_zero_of_width_one_denote_zero (e : Eqn) (h : (∀ env1 : List (BitVec 1), Eqn.denote e env1 = 0)) : 
+    ∀ (w : Nat) (env : List (BitVec w)), Eqn.reflect e env = 0 := by
+  intros w env
+  rw [Eqn.denote_hard_case]
+  exact h
 
 end MBA
 
